messages valid

ironfleet/ravana/Refinement.i.dfy
@@ -4,61 +4,86 @@ module Refinement_i {
   import opened Types_i
 
   predicate rstate_valid(rs: RState) {
-    true // TODO
+    packets_are_valid(rs)
   }
 
   function refinement(rs: RState) : ServiceState
   requires rstate_valid(rs)
   {
-    var log := rs.server_logger.log;
-
-    var (fwdControllerState, fwdOutstandingCommands) :=
-          controller_state_looking_forward(log, rs.initControllerState);
-
-    var curOutstandingCommands := set_to_multiset(set
-          command_id : int | (
-            0 <= command_id < |fwdOutstandingCommands| &&
-            var command := fwdOutstandingCommands[command_id];
-            command.switch in rs.server_switches &&
-            !(command_id in rs.server_switches[command.switch].received_command_ids)
-          ) ::
-            (command_id, fwdOutstandingCommands[command_id])
-        );
-
-    var switchStates := (
-      map switch : EndPoint
-      | switch in rs.server_switches
-      :: rs.server_switches[switch].switchState
-    );
-
-    var controllerState := fwdControllerState;
-    var outstandingCommands := curOutstandingCommands;
-
-    var outstandingEvents := set_to_multiset(set
-          switch : EndPoint, eid : int | (
-            switch in rs.server_switches &&
-            eid in rs.server_switches[switch].bufferedEvents
-          ) ::
-            ((switch, eid), SwitchEvent(switch, rs.server_switches[switch].bufferedEvents[eid]))
-        );
-
-    ServiceState(switchStates, controllerState, outstandingCommands, outstandingEvents)
+    ServiceState(
+      refinement_switchStates(rs.server_switches),
+      refinement_controllerState(rs.server_logger.log, rs.initControllerState),
+      refinement_outstandingCommands(rs.server_logger.log, rs.initControllerState,
+          rs.server_switches),
+      refinement_outstandingEvents(rs.server_switches, rs.server_logger.log)
+    )
   }
+
+  function refinement_switchStates(
+      server_switches: map<EndPoint, NodeSwitch>) : map<EndPoint, SwitchState>
+  {
+      map switch : EndPoint
+      | switch in server_switches
+      :: server_switches[switch].switchState
+  }
+
+  function refinement_outstandingEvents(
+      server_switches: map<EndPoint, NodeSwitch>,
+      log: seq<LogEntry>
+      ) : multiset<SwitchEvent>
+  {
+      set_to_multiset(set
+        switch : EndPoint, eid : int | (
+          switch in server_switches &&
+          eid in server_switches[switch].bufferedEvents &&
+          (forall entry :: entry in log ==>
+              !(entry.LMRecv? && entry.event_id == eid && entry.switch == switch))
+        ) ::
+          ((switch, eid), SwitchEvent(switch, server_switches[switch].bufferedEvents[eid]))
+      )
+  }
+
+  function refinement_controllerState(
+      log: seq<LogEntry>, initControllerState: ControllerState) : ControllerState
+  { 
+      controller_state_looking_forward(log, initControllerState).controllerState
+  }
+
+  function refinement_outstandingCommands(
+      log: seq<LogEntry>, initControllerState: ControllerState,
+      server_switches: map<EndPoint, NodeSwitch>) : multiset<SingleCommand>
+  {
+      var fwdOutstandingCommands := 
+          controller_state_looking_forward(log, initControllerState).commands;
+      set_to_multiset(set
+        command_id : int | (
+          0 <= command_id < |fwdOutstandingCommands| &&
+          var command := fwdOutstandingCommands[command_id];
+          command.switch in server_switches &&
+          !(command_id in server_switches[command.switch].received_command_ids)
+        ) ::
+          (command_id, fwdOutstandingCommands[command_id])
+      )
+  }
+
+  datatype StateAndCommands = StateAndCommands(
+      controllerState: ControllerState,
+      commands: seq<SingleCommand>)
 
   function controller_state_looking_forward(
       log: seq<LogEntry>,
-      controllerState: ControllerState) : (ControllerState, seq<SingleCommand>)
+      controllerState: ControllerState) : StateAndCommands
   {
     if |log| == 0 then
-      (controllerState, [])
+      StateAndCommands(controllerState, [])
     else (
-      var elem := log[0];
+      var elem := log[|log| - 1];
       if elem.LMProc? then (
-        controller_state_looking_forward(log[1 .. ], controllerState)
+        controller_state_looking_forward(log[0 .. |log| - 1], controllerState)
       ) else (
-        var (cs', comms1) := controllerTransition(controllerState, elem.switch, elem.event);
-        var (cs'', comms2) := controller_state_looking_forward(log[1 .. ], cs');
-        (cs'', comms1 + comms2)
+        var sac1 := controller_state_looking_forward(log[0 .. |log| - 1], controllerState);
+        var (cs'', commands) := controllerTransition(sac1.controllerState, elem.switch, elem.event);
+        StateAndCommands(cs'', sac1.commands + commands)
       )
     )
   }
@@ -73,5 +98,87 @@ module Refinement_i {
       var m' := m - {y};
       set_to_multiset(m') + multiset{b}
     )
+  }
+
+  predicate {:opaque} packets_are_valid(rs: RState)
+  {
+    (forall p :: p in rs.environment.sentPackets ==>
+        is_valid_message(rs, p.src, p.dst, p.msg))
+  }
+
+  predicate is_valid_message(rs: RState, src: EndPoint, dst: EndPoint, msg: RavanaMessage)
+  {
+    (msg.EventMessage? ==> is_valid_EventMessage(rs, src, dst, msg)) &&
+    (msg.EventAck? ==> is_valid_EventAck(rs, src, dst, msg)) &&
+    (msg.CommandMessage? ==> is_valid_CommandMessage(rs, src, dst, msg)) &&
+    (msg.CommandAck? ==> is_valid_CommandAck(rs, src, dst, msg)) &&
+    (msg.InitNewMaster? ==> is_valid_InitNewMaster(rs, src, dst, msg)) &&
+    (msg.NewMaster? ==> is_valid_NewMaster(rs, src, dst, msg)) &&
+    (msg.NewMasterAck? ==> is_valid_NewMasterAck(rs, src, dst, msg)) &&
+    (msg.LogMessage? ==> is_valid_LogMessage(rs, src, dst, msg)) &&
+    (msg.LogBroadcastMessage? ==> is_valid_LogBroadcastMessage(rs, src, dst, msg))
+  }
+
+  predicate is_valid_EventMessage(rs: RState, src: EndPoint, dst: EndPoint, msg: RavanaMessage)
+  requires msg.EventMessage?
+  {
+    true
+  }
+
+  predicate is_valid_EventAck(rs: RState, src: EndPoint, dst: EndPoint, msg: RavanaMessage)
+  requires msg.EventAck?
+  {
+    true
+  }
+
+  predicate is_valid_CommandMessage(rs: RState, src: EndPoint, dst: EndPoint, msg: RavanaMessage)
+  requires msg.CommandMessage?
+  {
+    true
+  }
+
+  predicate is_valid_CommandAck(rs: RState, src: EndPoint, dst: EndPoint, msg: RavanaMessage)
+  requires msg.CommandAck?
+  {
+    true
+  }
+
+  predicate is_valid_InitNewMaster(rs: RState, src: EndPoint, dst: EndPoint, msg: RavanaMessage)
+  requires msg.InitNewMaster?
+  {
+    true
+  }
+
+  predicate is_valid_NewMaster(rs: RState, src: EndPoint, dst: EndPoint, msg: RavanaMessage)
+  requires msg.NewMaster?
+  {
+    true
+  }
+
+  predicate is_valid_NewMasterAck(rs: RState, src: EndPoint, dst: EndPoint, msg: RavanaMessage)
+  requires msg.NewMasterAck?
+  {
+    true
+  }
+
+  predicate is_valid_LogMessage(rs: RState, src: EndPoint, dst: EndPoint, msg: RavanaMessage)
+  requires msg.LogMessage?
+  {
+    if (msg.log_entry.LMRecv?) then (
+      // LMRecv
+         msg.log_entry.switch in rs.server_switches
+      && msg.log_entry.event_id in rs.server_switches[msg.log_entry.switch].bufferedEvents
+      && rs.server_switches[msg.log_entry.switch].bufferedEvents[msg.log_entry.event_id] ==
+            msg.log_entry.event
+    ) else (
+      // LMProc
+      true
+    )
+  }
+
+  predicate is_valid_LogBroadcastMessage(rs: RState, src: EndPoint, dst: EndPoint, msg: RavanaMessage)
+  requires msg.LogBroadcastMessage?
+  {
+    true
   }
 }
