ironfleet/ravana/RefinementProof.i.dfy
@@ -21,19 +21,248 @@ module Refinement_Proof_i {
   }
   */
 
+  /*
   lemma lemma_refines_Logger_InitNewMaster(rs: RState, rs': RState)
   requires rstate_valid(rs)
 
   requires LEnvironment_Next(rs.environment, rs'.environment)
   requires rs.environment.nextStep.LEnvStepHostIos?
   requires rs.endpoint_logger == rs'.endpoint_logger
+  requires rs.initControllerState == rs'.initControllerState
   requires rs.environment.nextStep.actor == rs'.endpoint_logger
-  requires NodeNext_Logger(rs.server_logger, rs'.server_logger, rs.environment.nextStep.ios)
+  requires Node_LoggerInitNewMaster(
+              rs.server_logger, rs'.server_logger, rs.environment.nextStep.ios)
   requires rs.server_controllers == rs'.server_controllers
   requires rs.server_switches == rs'.server_switches
 
   ensures rstate_valid(rs')
   ensures refinement(rs) == refinement(rs')
   {
+    assert refinement_switchStates(rs.server_switches)
+        == refinement_switchStates(rs'.server_switches);
+
+    assert rs.server_logger.log == rs'.server_logger.log;
+
+    assert refinement_controllerState(rs.server_logger.log, rs.initControllerState)
+        == refinement_controllerState(rs'.server_logger.log, rs'.initControllerState);
+
+    assert refinement_outstandingCommands(rs.server_logger.log, rs.initControllerState, rs.server_switches)
+        == refinement_outstandingCommands(rs'.server_logger.log, rs'.initControllerState, rs'.server_switches);
+
+    assert refinement_outstandingEvents(rs.server_switches, rs.server_logger.log)
+        == refinement_outstandingEvents(rs'.server_switches, rs'.server_logger.log);
   }
+
+  lemma lemma_refines_Logger_InitNewMasterMsg(rs: RState, rs': RState)
+  requires rstate_valid(rs)
+
+  requires LEnvironment_Next(rs.environment, rs'.environment)
+  requires rs.environment.nextStep.LEnvStepHostIos?
+  requires rs.endpoint_logger == rs'.endpoint_logger
+  requires rs.initControllerState == rs'.initControllerState
+  requires rs.environment.nextStep.actor == rs'.endpoint_logger
+  requires Node_LoggerInitNewMasterMsg(
+              rs.server_logger, rs'.server_logger, rs.environment.nextStep.ios)
+  requires rs.server_controllers == rs'.server_controllers
+  requires rs.server_switches == rs'.server_switches
+
+  ensures rstate_valid(rs')
+  ensures refinement(rs) == refinement(rs')
+  {
+    
+  }
+
+  lemma lemma_refines_LoggerLogEvent(rs: RState, rs': RState)
+  requires rstate_valid(rs)
+
+  requires LEnvironment_Next(rs.environment, rs'.environment)
+  requires rs.environment.nextStep.LEnvStepHostIos?
+  requires rs.endpoint_logger == rs'.endpoint_logger
+  requires rs.initControllerState == rs'.initControllerState
+  requires rs.environment.nextStep.actor == rs'.endpoint_logger
+  requires Node_LoggerLogEvent(
+              rs.server_logger, rs'.server_logger, rs.environment.nextStep.ios)
+  requires rs.server_controllers == rs'.server_controllers
+  requires rs.server_switches == rs'.server_switches
+
+  ensures rstate_valid(rs')
+  ensures Service_NextApplyEvent(refinement(rs), refinement(rs'))
+       || refinement(rs) == refinement(rs')
+          
+  {
+    var s := refinement(rs);
+    var s' := refinement(rs');
+
+    assert rs.environment.nextStep.ios[0].LIoOpReceive?;
+    assert rs.environment.nextStep.ios[0].r.msg.LogMessage?;
+    var log_entry := rs.environment.nextStep.ios[0].r.msg.log_entry;
+
+    if (log_entry.LMRecv?) {
+      var switch_event := SwitchEvent(log_entry.switch, log_entry.event);
+
+      assert s.switchStates == s'.switchStates;
+
+      lemma_refines_LoggerLogEvent_multiset(rs, rs', log_entry);
+
+      assert multiset_adds_one(s'.outstandingEvents, s.outstandingEvents);
+      var event := added_obj(s'.outstandingEvents, s.outstandingEvents);
+      assert event == switch_event;
+
+      var cas := controllerTransition(s.controllerState, event.switch, event.event);
+      var cs' := cas.0;
+      var singleCommands := cas.1;
+
+      assert s'.controllerState == cs';
+      assert s'.outstandingCommands == s.outstandingCommands + seq_to_multiset(singleCommands);
+
+      assert Service_NextApplyEvent(refinement(rs), refinement(rs'));
+    } else {
+      assert s == s';
+    }
+  }
+  */
+
+  lemma lemma_refines_LoggerLogEvent_multiset(rs: RState, rs': RState, log_entry: LogEntry)
+  requires rstate_valid(rs)
+  requires LEnvironment_Next(rs.environment, rs'.environment)
+  requires rs.environment.nextStep.LEnvStepHostIos?
+  requires rs.endpoint_logger == rs'.endpoint_logger
+  requires rs.initControllerState == rs'.initControllerState
+  requires rs.environment.nextStep.actor == rs'.endpoint_logger
+  requires Node_LoggerLogEvent(
+              rs.server_logger, rs'.server_logger, rs.environment.nextStep.ios)
+  requires rs.server_controllers == rs'.server_controllers
+  requires rs.server_switches == rs'.server_switches
+
+  requires rs.environment.nextStep.ios[0].LIoOpReceive?;
+  requires rs.environment.nextStep.ios[0].r.msg.LogMessage?;
+  requires rs.environment.nextStep.ios[0].r.msg.log_entry == log_entry
+  requires log_entry.LMRecv?
+
+  ensures multiset_adds_one(refinement(rs').outstandingEvents, refinement(rs).outstandingEvents);
+  ensures SwitchEvent(log_entry.switch, log_entry.event)
+          == added_obj(refinement(rs').outstandingEvents, refinement(rs).outstandingEvents)
+  {
+    assert rs'.server_logger.log == rs.server_logger.log + [log_entry];
+    assert rs.server_switches == rs'.server_switches;
+
+    assert log_entry.switch in rs.server_switches;
+    assert log_entry.event_id in rs.server_switches[log_entry.switch].bufferedEvents;
+    assert rs.server_switches[log_entry.switch].bufferedEvents[log_entry.event_id]
+        == log_entry.event;
+
+    assert (forall entry :: entry in rs.server_logger.log ==>
+              !(entry.LMRecv? && entry.event_id == log_entry.event_id &&
+                  entry.switch == log_entry.switch));
+
+    assert 
+      (set
+        switch : EndPoint, eid : int | (
+          switch in rs.server_switches &&
+          eid in rs.server_switches[switch].bufferedEvents &&
+          (forall entry :: entry in rs.server_logger.log ==>
+              !(entry.LMRecv? && entry.event_id == eid && entry.switch == switch))
+        ) ::
+          ((switch, eid), SwitchEvent(switch, rs.server_switches[switch].bufferedEvents[eid]))
+      ) - (
+      set
+        switch : EndPoint, eid : int | (
+          switch in rs'.server_switches &&
+          eid in rs'.server_switches[switch].bufferedEvents &&
+          (forall entry :: entry in rs'.server_logger.log ==>
+              !(entry.LMRecv? && entry.event_id == eid && entry.switch == switch))
+        ) ::
+          ((switch, eid), SwitchEvent(switch, rs'.server_switches[switch].bufferedEvents[eid]))
+      )
+      ==
+      (set
+        switch : EndPoint, eid : int | (
+          switch in rs.server_switches &&
+          eid in rs.server_switches[switch].bufferedEvents &&
+          (forall entry :: entry in rs.server_logger.log ==>
+              !(entry.LMRecv? && entry.event_id == eid && entry.switch == switch))
+        ) ::
+          ((switch, eid), SwitchEvent(switch, rs.server_switches[switch].bufferedEvents[eid]))
+      ) - (
+      set
+        switch : EndPoint, eid : int | (
+          switch in rs.server_switches &&
+          eid in rs'.server_switches[switch].bufferedEvents &&
+          (forall entry :: entry in (rs.server_logger.log + [log_entry]) ==>
+              !(entry.LMRecv? && entry.event_id == eid && entry.switch == switch))
+        ) ::
+          ((switch, eid), SwitchEvent(switch, rs.server_switches[switch].bufferedEvents[eid]))
+      )
+      ==
+      (set
+        switch : EndPoint, eid : int | (
+          switch in rs.server_switches &&
+          eid in rs.server_switches[switch].bufferedEvents &&
+          (forall entry :: entry in rs.server_logger.log ==>
+              !(entry.LMRecv? && entry.event_id == eid && entry.switch == switch))
+          && !(
+            switch in rs.server_switches &&
+            eid in rs.server_switches[switch].bufferedEvents &&
+            (forall entry :: entry in (rs.server_logger.log + [log_entry]) ==>
+                !(entry.LMRecv? && entry.event_id == eid && entry.switch == switch))
+          )
+        ) ::
+          ((switch, eid), SwitchEvent(switch, rs.server_switches[switch].bufferedEvents[eid]))
+      )
+      ==
+      (set
+        switch : EndPoint, eid : int | (
+          switch in rs.server_switches &&
+          eid in rs.server_switches[switch].bufferedEvents &&
+          (forall entry :: entry in rs.server_logger.log ==>
+              !(entry.LMRecv? && entry.event_id == eid && entry.switch == switch))
+          && !(
+            (forall entry :: entry in (rs.server_logger.log + [log_entry]) ==>
+                !(entry.LMRecv? && entry.event_id == eid && entry.switch == switch))
+          )
+        ) ::
+          ((switch, eid), SwitchEvent(switch, rs.server_switches[switch].bufferedEvents[eid]))
+      )
+      ==
+      (set
+        switch : EndPoint, eid : int | (
+          switch in rs.server_switches &&
+          eid in rs.server_switches[switch].bufferedEvents &&
+          (forall entry :: entry in rs.server_logger.log ==>
+              !(entry.LMRecv? && entry.event_id == eid && entry.switch == switch))
+          && (log_entry.LMRecv? && log_entry.event_id == eid && log_entry.switch == switch)
+        ) ::
+          ((switch, eid), SwitchEvent(switch, rs.server_switches[switch].bufferedEvents[eid]))
+      )
+      ==
+      { ((log_entry.switch, log_entry.event_id),
+             SwitchEvent(log_entry.switch,
+             rs.server_switches[log_entry.switch].bufferedEvents[log_entry.event_id])) }
+      ==
+      { ((log_entry.switch, log_entry.event_id),
+             SwitchEvent(log_entry.switch, log_entry.event)) }
+      ;
+
+  }
+
+  /*
+  lemma lemma_refines_LoggerBroadcast(rs: RState, rs': RState)
+  requires rstate_valid(rs)
+
+  requires LEnvironment_Next(rs.environment, rs'.environment)
+  requires rs.environment.nextStep.LEnvStepHostIos?
+  requires rs.endpoint_logger == rs'.endpoint_logger
+  requires rs.initControllerState == rs'.initControllerState
+  requires rs.environment.nextStep.actor == rs'.endpoint_logger
+  requires Node_LoggerBroadcast(
+              rs.server_logger, rs'.server_logger, rs.environment.nextStep.ios)
+  requires rs.server_controllers == rs'.server_controllers
+  requires rs.server_switches == rs'.server_switches
+
+  ensures rstate_valid(rs')
+  ensures refinement(rs) == refinement(rs')
+  {
+
+  }
+  */
 }
